{
 "cells": [
  {
   "cell_type": "code",
   "execution_count": 1,
   "metadata": {},
   "outputs": [],
   "source": [
    "%matplotlib inline\n",
    "import matplotlib.pyplot as plt\n",
    "import matplotlib.animation as animation\n",
    "from IPython.display import HTML\n",
    "\n",
    "import numpy as np\n",
    "import numpy.linalg as la\n",
    "from scipy.integrate import RK45\n",
    "\n",
    "import sympy as sym\n",
    "# Heaviside numerics workaround\n",
    "sympy_modules = [{'Heaviside': lambda x: np.heaviside(x,0.5)}, 'numpy']\n",
    "\n",
    "from table_maker import *\n",
    "from functools import partial, reduce\n",
    "from itertools import *\n",
    "from math import ceil\n",
    "\n",
    "import pickle\n",
    "\n",
    "def cos_bell(x, center=0, width=2*np.pi, height=1):\n",
    "    return (np.cos((x-center)/width*2*np.pi)+1)/2*height * np.heaviside(x-center+width/2,0) * np.heaviside(-x+center+width/2,0)\n",
    "\n",
    "import collections.abc\n",
    "def collect_eqn(expr, terms):\n",
    "    if not isinstance(terms, collections.abc.Container):\n",
    "        term = terms # isn't a list or tuple\n",
    "        left, right = 0,0\n",
    "        for my_expr in expr.args:\n",
    "            has_term = False\n",
    "            for my_term in sym.postorder_traversal(my_expr):\n",
    "                if term == my_term:\n",
    "                    has_term = True\n",
    "                    break\n",
    "            if has_term:\n",
    "                left += my_expr\n",
    "            else:\n",
    "                right -= my_expr\n",
    "        return sym.Eq(left, right, evaluate=False)\n",
    "    else: # isn't a list or tuple\n",
    "        left_total, right_total = 0, expr\n",
    "        for term in terms:\n",
    "            left, right = collect_eqn(right_total, term).args\n",
    "            left_total += left\n",
    "            right_total = -right\n",
    "        return sym.Eq(left_total, right_total, evaluate=False)\n",
    "    \n",
    "def my_print(expr):\n",
    "    global eviron_print_tex\n",
    "    if eviron_print_tex:\n",
    "        print('$$' + sym.latex(expr) + '$$')\n",
    "    else:\n",
    "        display(expr)\n",
    "        \n",
    "def batch_print(expr_list, punctuation='.', return_string=False):\n",
    "    global eviron_print_tex\n",
    "    if eviron_print_tex:\n",
    "        print_str = '$$\\\\begin{align*}\\n'\n",
    "        for expr in expr_list:\n",
    "            print_str += '\\t' + sym.latex(expr).replace('=','&=') + '\\\\\\\\\\n'\n",
    "        # remove last new-line and add ending puncuation\n",
    "        print_str = print_str[:-3] + punctuation + '\\n'\n",
    "        print_str += '\\\\end{align*}$$'\n",
    "        if return_string:\n",
    "            return print_str\n",
    "        else:\n",
    "            print(print_str)\n",
    "    else:\n",
    "        for expr in expr_list:\n",
    "            display(expr)\n",
    "            \n",
    "def py_code(expr, replace_numpy=True, replace_unicode=True, numpy_package='np.'):\n",
    "    code = sym.ccode(expr)\n",
    "    \n",
    "    if replace_unicode:\n",
    "        unicode_replacements = [\n",
    "            ('\\\\alpha', 'α'),\n",
    "            ('\\\\beta', 'β'),\n",
    "            ('\\\\gamma', 'γ'),\n",
    "            ('\\\\Gamma', 'Γ'),\n",
    "            ('\\\\delta', 'δ'),\n",
    "            ('\\\\Delta', 'Δ'),\n",
    "            ('\\\\epsilon', 'ϵ'),\n",
    "            ('\\\\zeta', 'ζ'),\n",
    "            ('\\\\eta', 'η'),\n",
    "            ('\\\\theta', 'θ'),\n",
    "            ('\\\\xi', 'ξ'),\n",
    "            ('\\\\mu', 'μ')\n",
    "        ]\n",
    "        for unicode, symbol in unicode_replacements:\n",
    "            code = code.replace(unicode, symbol)\n",
    "    \n",
    "    if replace_numpy:\n",
    "        numpy_replacements = [\n",
    "            ('exp', numpy_package + 'exp'),\n",
    "            ('log', numpy_package + 'log'),\n",
    "            ('pow', '( lambda base, exponent: base**exponent )'),\n",
    "            ('Heaviside', '(lambda input: np.heaviside(input,0.5))')\n",
    "        ]\n",
    "        for c_func, np_func in numpy_replacements:\n",
    "            code = code.replace(c_func, np_func)\n",
    "        \n",
    "    return code"
   ]
  },
  {
   "cell_type": "code",
   "execution_count": 2,
   "metadata": {},
   "outputs": [],
   "source": [
    "import matplotlib\n",
    "matplotlib.rcParams.update({'font.size': 24})"
   ]
  },
  {
   "cell_type": "code",
   "execution_count": 155,
   "metadata": {},
   "outputs": [
    {
     "name": "stdout",
     "output_type": "stream",
     "text": [
      "Solving the system, we obtain the solution in terms of 7 unkown constants\n",
      "$$\\begin{align*}\n",
      "\tU{\\left(\\xi \\right)} &= \\begin{cases} C_{1} e^{\\frac{\\xi}{\\mu c}} + \\frac{\\left(\\frac{1}{2} + \\frac{\\left(\\frac{e^{\\Delta}}{2} - \\frac{1}{2}\\right) e^{- \\lambda}}{1 - e^{- \\lambda}}\\right) e^{\\xi}}{- \\mu c + 1} + \\frac{\\left(\\frac{\\left(\\frac{1}{2} - \\frac{e^{- \\Delta}}{2}\\right) e^{- \\lambda}}{1 - e^{- \\lambda}} - \\frac{e^{- \\Delta}}{2}\\right) e^{- \\xi}}{\\mu c + 1} & \\text{for}\\: \\xi < 0 \\\\C_{2} e^{\\frac{\\xi}{\\mu c}} + \\frac{\\left(\\frac{1}{2} - \\frac{e^{- \\Delta}}{2}\\right) e^{- \\xi}}{\\left(1 - e^{- \\lambda}\\right) \\left(\\mu c + 1\\right)} + \\frac{\\left(\\frac{e^{\\Delta}}{2} - \\frac{1}{2}\\right) e^{- \\lambda} e^{\\xi}}{\\left(1 - e^{- \\lambda}\\right) \\left(- \\mu c + 1\\right)} & \\text{otherwise} \\end{cases}\\\\\n",
      "\tA{\\left(\\xi \\right)} &= \\begin{cases} C_{3} e^{\\frac{\\xi}{\\alpha c}} + \\gamma & \\text{for}\\: \\xi < 0 \\\\C_{4} e^{\\frac{\\xi}{\\alpha c}} & \\text{otherwise} \\end{cases}.\n",
      "\\end{align*}$$\n",
      "Enforcing continuity of $U$ at $\\xi=0$ and over the boundary $\\xi = -\\Delta, \\lambda-\\Delta$ we obtain the following equations for $C_1$ and $C_2$\n",
      "$$\n",
      "\\left[\\begin{matrix}1 & -1\\\\e^{- \\frac{\\Delta}{\\mu c}} & - e^{\\frac{- \\Delta + \\lambda}{\\mu c}}\\end{matrix}\\right]\\left[\\begin{matrix}C_{1}\\\\C_{2}\\end{matrix}\\right]=\\left[\\begin{matrix}- \\frac{\\frac{1}{2} + \\frac{\\left(\\frac{e^{\\Delta}}{2} - \\frac{1}{2}\\right) e^{- \\lambda}}{1 - e^{- \\lambda}}}{- \\mu c + 1} + \\frac{\\frac{1}{2} - \\frac{e^{- \\Delta}}{2}}{\\left(1 - e^{- \\lambda}\\right) \\left(\\mu c + 1\\right)} - \\frac{\\frac{\\left(\\frac{1}{2} - \\frac{e^{- \\Delta}}{2}\\right) e^{- \\lambda}}{1 - e^{- \\lambda}} - \\frac{e^{- \\Delta}}{2}}{\\mu c + 1} + \\frac{\\left(\\frac{e^{\\Delta}}{2} - \\frac{1}{2}\\right) e^{- \\lambda}}{\\left(1 - e^{- \\lambda}\\right) \\left(- \\mu c + 1\\right)}\\\\- \\frac{\\left(\\frac{1}{2} + \\frac{\\left(\\frac{e^{\\Delta}}{2} - \\frac{1}{2}\\right) e^{- \\lambda}}{1 - e^{- \\lambda}}\\right) e^{- \\Delta}}{- \\mu c + 1} + \\frac{\\left(\\frac{1}{2} - \\frac{e^{- \\Delta}}{2}\\right) e^{\\Delta - \\lambda}}{\\left(1 - e^{- \\lambda}\\right) \\left(\\mu c + 1\\right)} - \\frac{\\left(\\frac{\\left(\\frac{1}{2} - \\frac{e^{- \\Delta}}{2}\\right) e^{- \\lambda}}{1 - e^{- \\lambda}} - \\frac{e^{- \\Delta}}{2}\\right) e^{\\Delta}}{\\mu c + 1} + \\frac{\\left(\\frac{e^{\\Delta}}{2} - \\frac{1}{2}\\right) e^{- \\lambda} e^{- \\Delta + \\lambda}}{\\left(1 - e^{- \\lambda}\\right) \\left(- \\mu c + 1\\right)}\\end{matrix}\\right]\n",
      "$$\n",
      "which gives\n",
      "$$\\begin{align*}\n",
      "\tC_{1} &= - \\frac{\\left(- \\frac{\\frac{1}{2} + \\frac{\\left(\\frac{e^{\\Delta}}{2} - \\frac{1}{2}\\right) e^{- \\lambda}}{1 - e^{- \\lambda}}}{- \\mu c + 1} + \\frac{\\frac{1}{2} - \\frac{e^{- \\Delta}}{2}}{\\left(1 - e^{- \\lambda}\\right) \\left(\\mu c + 1\\right)} - \\frac{\\frac{\\left(\\frac{1}{2} - \\frac{e^{- \\Delta}}{2}\\right) e^{- \\lambda}}{1 - e^{- \\lambda}} - \\frac{e^{- \\Delta}}{2}}{\\mu c + 1} + \\frac{\\left(\\frac{e^{\\Delta}}{2} - \\frac{1}{2}\\right) e^{- \\lambda}}{\\left(1 - e^{- \\lambda}\\right) \\left(- \\mu c + 1\\right)}\\right) e^{- \\frac{\\Delta}{\\mu c} + \\frac{\\lambda}{\\mu c}}}{- e^{- \\frac{\\Delta}{\\mu c} + \\frac{\\lambda}{\\mu c}} + e^{- \\frac{\\Delta}{\\mu c}}} + \\frac{- \\frac{\\left(\\frac{1}{2} + \\frac{\\left(\\frac{e^{\\Delta}}{2} - \\frac{1}{2}\\right) e^{- \\lambda}}{1 - e^{- \\lambda}}\\right) e^{- \\Delta}}{- \\mu c + 1} + \\frac{\\left(\\frac{1}{2} - \\frac{e^{- \\Delta}}{2}\\right) e^{\\Delta - \\lambda}}{\\left(1 - e^{- \\lambda}\\right) \\left(\\mu c + 1\\right)} - \\frac{\\left(\\frac{\\left(\\frac{1}{2} - \\frac{e^{- \\Delta}}{2}\\right) e^{- \\lambda}}{1 - e^{- \\lambda}} - \\frac{e^{- \\Delta}}{2}\\right) e^{\\Delta}}{\\mu c + 1} + \\frac{\\left(\\frac{e^{\\Delta}}{2} - \\frac{1}{2}\\right) e^{- \\lambda} e^{- \\Delta + \\lambda}}{\\left(1 - e^{- \\lambda}\\right) \\left(- \\mu c + 1\\right)}}{- e^{- \\frac{\\Delta}{\\mu c} + \\frac{\\lambda}{\\mu c}} + e^{- \\frac{\\Delta}{\\mu c}}}\\\\\n",
      "\tC_{2} &= \\frac{- \\frac{\\left(\\frac{1}{2} + \\frac{\\left(\\frac{e^{\\Delta}}{2} - \\frac{1}{2}\\right) e^{- \\lambda}}{1 - e^{- \\lambda}}\\right) e^{- \\Delta}}{- \\mu c + 1} + \\frac{\\left(\\frac{1}{2} - \\frac{e^{- \\Delta}}{2}\\right) e^{\\Delta - \\lambda}}{\\left(1 - e^{- \\lambda}\\right) \\left(\\mu c + 1\\right)} - \\frac{\\left(\\frac{\\left(\\frac{1}{2} - \\frac{e^{- \\Delta}}{2}\\right) e^{- \\lambda}}{1 - e^{- \\lambda}} - \\frac{e^{- \\Delta}}{2}\\right) e^{\\Delta}}{\\mu c + 1} + \\frac{\\left(\\frac{e^{\\Delta}}{2} - \\frac{1}{2}\\right) e^{- \\lambda} e^{- \\Delta + \\lambda}}{\\left(1 - e^{- \\lambda}\\right) \\left(- \\mu c + 1\\right)}}{- e^{- \\frac{\\Delta}{\\mu c} + \\frac{\\lambda}{\\mu c}} + e^{- \\frac{\\Delta}{\\mu c}}} - \\frac{- \\frac{\\frac{1}{2} + \\frac{\\left(\\frac{e^{\\Delta}}{2} - \\frac{1}{2}\\right) e^{- \\lambda}}{1 - e^{- \\lambda}}}{- \\mu c + 1} + \\frac{\\frac{1}{2} - \\frac{e^{- \\Delta}}{2}}{\\left(1 - e^{- \\lambda}\\right) \\left(\\mu c + 1\\right)} - \\frac{\\frac{\\left(\\frac{1}{2} - \\frac{e^{- \\Delta}}{2}\\right) e^{- \\lambda}}{1 - e^{- \\lambda}} - \\frac{e^{- \\Delta}}{2}}{\\mu c + 1} + \\frac{\\left(\\frac{e^{\\Delta}}{2} - \\frac{1}{2}\\right) e^{- \\lambda}}{\\left(1 - e^{- \\lambda}\\right) \\left(- \\mu c + 1\\right)}}{- e^{\\frac{\\Delta}{\\mu c}} e^{- \\frac{\\Delta}{\\mu c} + \\frac{\\lambda}{\\mu c}} + 1}.\n",
      "\\end{align*}$$\n",
      "Enforcing continuity of $A$ at $\\xi=0$ and over the boundary $\\xi = -\\Delta, \\lambda-\\Delta$ we obtain the following equations for $C_3$ and $C_4$\n",
      "$$\n",
      "\\left[\\begin{matrix}1 & -1\\\\e^{- \\frac{\\Delta}{\\alpha c}} & - e^{\\frac{- \\Delta + \\lambda}{\\alpha c}}\\end{matrix}\\right]\\left[\\begin{matrix}C_{3}\\\\C_{4}\\end{matrix}\\right]=\\left[\\begin{matrix}- \\gamma\\\\- \\gamma\\end{matrix}\\right]\n",
      "$$\n",
      "which gives\n",
      "$$\\begin{align*}\n",
      "\tC_{3} &= \\frac{\\gamma e^{- \\frac{\\Delta}{\\alpha c} + \\frac{\\lambda}{\\alpha c}}}{- e^{- \\frac{\\Delta}{\\alpha c} + \\frac{\\lambda}{\\alpha c}} + e^{- \\frac{\\Delta}{\\alpha c}}} - \\frac{\\gamma}{- e^{- \\frac{\\Delta}{\\alpha c} + \\frac{\\lambda}{\\alpha c}} + e^{- \\frac{\\Delta}{\\alpha c}}}\\\\\n",
      "\tC_{4} &= - \\frac{\\gamma}{- e^{- \\frac{\\Delta}{\\alpha c} + \\frac{\\lambda}{\\alpha c}} + e^{- \\frac{\\Delta}{\\alpha c}}} + \\frac{\\gamma}{- e^{\\frac{\\Delta}{\\alpha c}} e^{- \\frac{\\Delta}{\\alpha c} + \\frac{\\lambda}{\\alpha c}} + 1}.\n",
      "\\end{align*}$$\n",
      "We now have the solution in terms of $\\lambda, \\Delta$ and $c$. Enforcing threshold crossing of $U-A$ at $\\xi = 0, -\\Delta$ gives\n",
      "$$\\begin{align*}\n",
      "\t0 &= \\frac{\\gamma}{- e^{- \\frac{\\Delta}{\\alpha c} + \\frac{\\lambda}{\\alpha c}} + e^{- \\frac{\\Delta}{\\alpha c}}} - \\frac{\\gamma}{- e^{\\frac{\\Delta}{\\alpha c}} e^{- \\frac{\\Delta}{\\alpha c} + \\frac{\\lambda}{\\alpha c}} + 1} - \\theta + \\frac{\\frac{1}{2} - \\frac{e^{- \\Delta}}{2}}{\\left(1 - e^{- \\lambda}\\right) \\left(\\mu c + 1\\right)} + \\frac{- \\frac{\\left(\\frac{1}{2} + \\frac{\\left(\\frac{e^{\\Delta}}{2} - \\frac{1}{2}\\right) e^{- \\lambda}}{1 - e^{- \\lambda}}\\right) e^{- \\Delta}}{- \\mu c + 1} + \\frac{\\left(\\frac{1}{2} - \\frac{e^{- \\Delta}}{2}\\right) e^{\\Delta - \\lambda}}{\\left(1 - e^{- \\lambda}\\right) \\left(\\mu c + 1\\right)} - \\frac{\\left(\\frac{\\left(\\frac{1}{2} - \\frac{e^{- \\Delta}}{2}\\right) e^{- \\lambda}}{1 - e^{- \\lambda}} - \\frac{e^{- \\Delta}}{2}\\right) e^{\\Delta}}{\\mu c + 1} + \\frac{\\left(\\frac{e^{\\Delta}}{2} - \\frac{1}{2}\\right) e^{- \\lambda} e^{- \\Delta + \\lambda}}{\\left(1 - e^{- \\lambda}\\right) \\left(- \\mu c + 1\\right)}}{- e^{- \\frac{\\Delta}{\\mu c} + \\frac{\\lambda}{\\mu c}} + e^{- \\frac{\\Delta}{\\mu c}}} - \\frac{- \\frac{\\frac{1}{2} + \\frac{\\left(\\frac{e^{\\Delta}}{2} - \\frac{1}{2}\\right) e^{- \\lambda}}{1 - e^{- \\lambda}}}{- \\mu c + 1} + \\frac{\\frac{1}{2} - \\frac{e^{- \\Delta}}{2}}{\\left(1 - e^{- \\lambda}\\right) \\left(\\mu c + 1\\right)} - \\frac{\\frac{\\left(\\frac{1}{2} - \\frac{e^{- \\Delta}}{2}\\right) e^{- \\lambda}}{1 - e^{- \\lambda}} - \\frac{e^{- \\Delta}}{2}}{\\mu c + 1} + \\frac{\\left(\\frac{e^{\\Delta}}{2} - \\frac{1}{2}\\right) e^{- \\lambda}}{\\left(1 - e^{- \\lambda}\\right) \\left(- \\mu c + 1\\right)}}{- e^{\\frac{\\Delta}{\\mu c}} e^{- \\frac{\\Delta}{\\mu c} + \\frac{\\lambda}{\\mu c}} + 1} + \\frac{\\left(\\frac{e^{\\Delta}}{2} - \\frac{1}{2}\\right) e^{- \\lambda}}{\\left(1 - e^{- \\lambda}\\right) \\left(- \\mu c + 1\\right)}\\\\\n",
      "\t0 &= - \\theta + \\frac{\\left(\\frac{1}{2} - \\frac{e^{- \\Delta}}{2}\\right) e^{\\Delta}}{\\left(1 - e^{- \\lambda}\\right) \\left(\\mu c + 1\\right)} - \\left(- \\frac{\\gamma}{- e^{- \\frac{\\Delta}{\\alpha c} + \\frac{\\lambda}{\\alpha c}} + e^{- \\frac{\\Delta}{\\alpha c}}} + \\frac{\\gamma}{- e^{\\frac{\\Delta}{\\alpha c}} e^{- \\frac{\\Delta}{\\alpha c} + \\frac{\\lambda}{\\alpha c}} + 1}\\right) e^{- \\frac{\\Delta}{\\alpha c}} + \\left(\\frac{- \\frac{\\left(\\frac{1}{2} + \\frac{\\left(\\frac{e^{\\Delta}}{2} - \\frac{1}{2}\\right) e^{- \\lambda}}{1 - e^{- \\lambda}}\\right) e^{- \\Delta}}{- \\mu c + 1} + \\frac{\\left(\\frac{1}{2} - \\frac{e^{- \\Delta}}{2}\\right) e^{\\Delta - \\lambda}}{\\left(1 - e^{- \\lambda}\\right) \\left(\\mu c + 1\\right)} - \\frac{\\left(\\frac{\\left(\\frac{1}{2} - \\frac{e^{- \\Delta}}{2}\\right) e^{- \\lambda}}{1 - e^{- \\lambda}} - \\frac{e^{- \\Delta}}{2}\\right) e^{\\Delta}}{\\mu c + 1} + \\frac{\\left(\\frac{e^{\\Delta}}{2} - \\frac{1}{2}\\right) e^{- \\lambda} e^{- \\Delta + \\lambda}}{\\left(1 - e^{- \\lambda}\\right) \\left(- \\mu c + 1\\right)}}{- e^{- \\frac{\\Delta}{\\mu c} + \\frac{\\lambda}{\\mu c}} + e^{- \\frac{\\Delta}{\\mu c}}} - \\frac{- \\frac{\\frac{1}{2} + \\frac{\\left(\\frac{e^{\\Delta}}{2} - \\frac{1}{2}\\right) e^{- \\lambda}}{1 - e^{- \\lambda}}}{- \\mu c + 1} + \\frac{\\frac{1}{2} - \\frac{e^{- \\Delta}}{2}}{\\left(1 - e^{- \\lambda}\\right) \\left(\\mu c + 1\\right)} - \\frac{\\frac{\\left(\\frac{1}{2} - \\frac{e^{- \\Delta}}{2}\\right) e^{- \\lambda}}{1 - e^{- \\lambda}} - \\frac{e^{- \\Delta}}{2}}{\\mu c + 1} + \\frac{\\left(\\frac{e^{\\Delta}}{2} - \\frac{1}{2}\\right) e^{- \\lambda}}{\\left(1 - e^{- \\lambda}\\right) \\left(- \\mu c + 1\\right)}}{- e^{\\frac{\\Delta}{\\mu c}} e^{- \\frac{\\Delta}{\\mu c} + \\frac{\\lambda}{\\mu c}} + 1}\\right) e^{- \\frac{\\Delta}{\\mu c}} + \\frac{\\left(\\frac{e^{\\Delta}}{2} - \\frac{1}{2}\\right) e^{- \\Delta} e^{- \\lambda}}{\\left(1 - e^{- \\lambda}\\right) \\left(- \\mu c + 1\\right)}.\n",
      "\\end{align*}$$\n"
     ]
    }
   ],
   "source": [
    "eviron_print_tex = True\n",
    "\n",
    "μ, α, γ, θ, c, Δ, λ = sym.symbols('\\\\mu \\\\alpha \\\\gamma, \\\\theta, c \\\\Delta \\\\lambda', real=True, positive = True)\n",
    "\n",
    "ξ = sym.symbols('\\\\xi', real=True)\n",
    "\n",
    "U = sym.Function('U', real=True)(ξ)\n",
    "A = sym.Function('A', real=True)(ξ)\n",
    "\n",
    "LU = lambda f: c*μ*f.diff(ξ) - f\n",
    "LA = lambda f: c*α*f.diff(ξ) - f\n",
    "\n",
    "coeff_left_pos = (sym.exp(Δ) - 1)/2 * sym.exp(-λ)/(1-sym.exp(-λ)) + sym.Rational(1,2)\n",
    "coeff_left_neg = (1 - sym.exp(-Δ))/2 * sym.exp(-λ)/(1-sym.exp(-λ)) - sym.exp(-Δ)/2\n",
    "F_left = coeff_left_pos * sym.exp(ξ) + coeff_left_neg*sym.exp(-ξ)\n",
    "\n",
    "coeff_right_pos = (sym.exp(Δ)-1)/2*sym.exp(-λ)/(1-sym.exp(-λ))\n",
    "coeff_right_neg = (1-sym.exp(-Δ))/2/(1-sym.exp(-λ))\n",
    "F_right = coeff_right_pos * sym.exp(ξ) + coeff_right_neg*sym.exp(-ξ)\n",
    "\n",
    "G_left = γ\n",
    "G_right = 0\n",
    "\n",
    "# homogeneous\n",
    "Uhom = sym.dsolve(LU(U), U).args[1]\n",
    "Ahom = sym.dsolve(LA(A), A).args[1]\n",
    "B, C = sym.symbols('B C', real=True)\n",
    "C1, C2, C3, C4 = sym.symbols('C1 C2 C3 C4')\n",
    "\n",
    "# U left\n",
    "ansatz = B*sym.exp(ξ) + C*sym.exp(-ξ)\n",
    "L_ansatz = LU(ansatz).expand().collect(sym.exp(ξ))\n",
    "B_sub = coeff_left_pos/-L_ansatz.collect(B).coeff(B*sym.exp(ξ))\n",
    "C_sub = coeff_left_neg/-L_ansatz.collect(C).coeff(C*sym.exp(-ξ))\n",
    "U_particular_left = B_sub*sym.exp(ξ) + C_sub*sym.exp(-ξ)\n",
    "assert (LU(U_particular_left) + F_left).simplify() == 0\n",
    "U_left = Uhom.expand().subs(sym.exp(C1/μ/c), C1) + U_particular_left\n",
    "\n",
    "# U right\n",
    "ansatz = B*sym.exp(ξ) + C*sym.exp(-ξ)\n",
    "L_ansatz = LU(ansatz).expand().collect(sym.exp(ξ))\n",
    "B_sub = coeff_right_pos/-L_ansatz.collect(B).coeff(B*sym.exp(ξ))\n",
    "C_sub = coeff_right_neg/-L_ansatz.collect(C).coeff(C*sym.exp(-ξ))\n",
    "U_particular_right = B_sub*sym.exp(ξ) + C_sub*sym.exp(-ξ)\n",
    "assert (LU(U_particular_right) + F_right).simplify() == 0\n",
    "U_right = Uhom.expand().subs(sym.exp(C1/μ/c), C2) + U_particular_right\n",
    "\n",
    "# A left\n",
    "L_ansatz = LA(B)\n",
    "B_sub = G_left/-L_ansatz.coeff(B)\n",
    "A_particular_left = B_sub\n",
    "assert (LA(A_particular_left) + G_left).simplify() == 0\n",
    "A_left = Ahom.expand().subs(sym.exp(C1/α/c), C3) + A_particular_left\n",
    "\n",
    "# A right\n",
    "A_right = Ahom.expand().subs(sym.exp(C1/α/c), C4)\n",
    "\n",
    "# piecewise - for printing\n",
    "U_piecewise = sym.Piecewise( (U_left, ξ<0), (U_right, 0<= ξ) )\n",
    "A_piecewise = sym.Piecewise( (A_left, ξ<0), (A_right, 0<= ξ) )\n",
    "\n",
    "print('Solving the system, we obtain the solution in terms of 7 unkown constants')\n",
    "batch_print([ sym.Eq(U, U_piecewise), sym.Eq(A, A_piecewise) ])\n",
    "\n",
    "expr1 = U_left.subs(ξ,0) - U_right.subs(ξ,0)\n",
    "row1 = [expr1.coeff(C1), expr1.coeff(C2)]\n",
    "rhs1 = row1[0]*C1 + row1[1]*C2 - expr1\n",
    "\n",
    "expr2 = U_left.subs(ξ,-Δ) - U_right.subs(ξ,λ-Δ)\n",
    "row2 = [expr2.coeff(C1), expr2.coeff(C2)]\n",
    "rhs2 = row2[0]*C1 + row2[1]*C2 - expr2\n",
    "\n",
    "mat = sym.Matrix([row1, row2])\n",
    "rhs = sym.Matrix([[rhs1], [rhs2]])\n",
    "\n",
    "print('Enforcing continuity of $U$ at $\\\\xi=0$ and over the boundary $\\\\xi = -\\\\Delta, \\\\lambda-\\\\Delta$ we obtain the following equations for $C_1$ and $C_2$')\n",
    "print('$$')\n",
    "print(sym.latex(mat) + sym.latex(sym.Matrix([[C1],[C2]])) + '=' + sym.latex(rhs))\n",
    "print('$$')\n",
    "\n",
    "C1_sub, C2_sub = mat**-1 * rhs\n",
    "\n",
    "print('which gives')\n",
    "batch_print([sym.Eq(C1, C1_sub), sym.Eq(C2, C2_sub)])\n",
    "\n",
    "expr1 = A_left.subs(ξ,0) - A_right.subs(ξ,0)\n",
    "row1 = [expr1.coeff(C3), expr1.coeff(C4)]\n",
    "rhs1 = row1[0]*C3 + row1[1]*C4 - expr1\n",
    "\n",
    "expr2 = A_left.subs(ξ,-Δ) - A_right.subs(ξ,λ-Δ)\n",
    "row2 = [expr2.coeff(C3), expr2.coeff(C4)]\n",
    "rhs2 = row2[0]*C3 + row2[1]*C4 - expr2\n",
    "\n",
    "mat = sym.Matrix([row1, row2])\n",
    "rhs = sym.Matrix([[rhs1], [rhs2]])\n",
    "\n",
    "print('Enforcing continuity of $A$ at $\\\\xi=0$ and over the boundary $\\\\xi = -\\\\Delta, \\\\lambda-\\\\Delta$ we obtain the following equations for $C_3$ and $C_4$')\n",
    "print('$$')\n",
    "print(sym.latex(mat) + sym.latex(sym.Matrix([[C3],[C4]])) + '=' + sym.latex(rhs))\n",
    "print('$$')\n",
    "\n",
    "C3_sub, C4_sub = mat**-1 * rhs\n",
    "\n",
    "print('which gives')\n",
    "batch_print([sym.Eq(C3, C3_sub), sym.Eq(C4, C4_sub)])\n",
    "\n",
    "print('We now have the solution in terms of $\\\\lambda, \\\\Delta$ and $c$. Enforcing threshold crossing of $U-A$ at $\\\\xi = 0, -\\\\Delta$ gives')\n",
    "cond1 = (U_right - A_right - θ).subs({ξ:0, C2:C2_sub, C4:C4_sub})\n",
    "cond2 = (U_right - A_right - θ).subs({ξ:-Δ, C2:C2_sub, C4:C4_sub})\n",
    "batch_print([sym.Eq(0,cond1), sym.Eq(0,cond2)])"
   ]
  },
  {
   "cell_type": "code",
   "execution_count": null,
   "metadata": {},
   "outputs": [],
   "source": []
  }
 ],
 "metadata": {
  "kernelspec": {
   "display_name": "Python 3",
   "language": "python",
   "name": "python3"
  },
  "language_info": {
   "codemirror_mode": {
    "name": "ipython",
    "version": 3
   },
   "file_extension": ".py",
   "mimetype": "text/x-python",
   "name": "python",
   "nbconvert_exporter": "python",
   "pygments_lexer": "ipython3",
   "version": "3.6.9"
  }
 },
 "nbformat": 4,
 "nbformat_minor": 4
}
